Fixed the quantifier puller. It was still using the old version of type denotations that took a type list as argumetns.

MirrorCharge!/src/MirrorCharge/ILPullQuant2.v
@@ -39,7 +39,7 @@ Section ILPullQuant.
   
 Require Import Charge.Logics.ILogic.
   
-  Variable inhabited_sound : forall t ts, inhabited t = true -> Inhabited (typD ts t).
+  Variable inhabited_sound : forall t, inhabited t = true -> Inhabited (typD t).
 
 Let Rbase := expr typ func.
 
@@ -232,13 +232,13 @@ Inductive typ :=
 | tyNat | tyBool | tyEmpty
 | tyProp.
 
-Fixpoint typD (ts : list Type) (t : typ) : Type :=
+Fixpoint typD (t : typ) : Type :=
   match t with
     | tyNat => nat
     | tyBool => bool
     | tyProp => Prop
     | tyEmpty => Empty_set
-    | tyArr a b => typD ts a -> typD ts b
+    | tyArr a b => typD a -> typD b
   end.
 
 Definition typ_eq_dec : forall a b : typ, {a = b} + {a <> b}.
@@ -267,7 +267,7 @@ Inductive tyAcc' : typ -> typ -> Prop :=
 Instance RType_typ : RType typ :=
 { typD := typD
 ; tyAcc := tyAcc'
-; type_cast := fun _ a b => match typ_eq_dec a b with
+; type_cast := fun a b => match typ_eq_dec a b with
                               | left pf => Some pf
                               | _ => None
                             end
@@ -290,10 +290,10 @@ Qed.
 
 Instance Typ2_tyArr : Typ2 _ Fun :=
 { typ2 := tyArr
-; typ2_cast := fun _ _ _ => eq_refl
-; typ2_match :=
-    fun T ts t tr =>
-      match t as t return T (TypesI.typD ts t) -> T (TypesI.typD ts t) with
+; typ2_cast := fun _ _ => eq_refl
+; typ2_match := 
+    fun T t tr =>
+      match t as t return T (TypesI.typD t) -> T (TypesI.typD t) with
         | tyArr a b => fun _ => tr a b
         | _ => fun fa => fa
       end
@@ -313,10 +313,10 @@ Qed.
 
 Instance Typ0_tyProp : Typ0 _ Prop :=
 {| typ0 := tyProp
- ; typ0_cast := fun _ => eq_refl
- ; typ0_match := fun T ts t =>
+ ; typ0_cast := eq_refl
+ ; typ0_match := fun T t =>
                    match t as t
-                         return T Prop -> T (TypesI.typD ts t) -> T (TypesI.typD ts t)
+                         return T Prop -> T (TypesI.typD t) -> T (TypesI.typD t)
                    with
                      | tyProp => fun tr _ => tr
                      | _ => fun _ fa => fa
@@ -332,14 +332,14 @@ Definition typeof_func (f : func) : option typ :=
          | Eq t => tyArr t (tyArr t tyProp)
        end.
 
-Definition funcD (ts : list Type) (f : func)
+Definition funcD (f : func)
 : match typeof_func f with
     | None => unit
-    | Some t => typD ts t
+    | Some t => typD t
   end :=
   match f as f return match typeof_func f with
                         | None => unit
-                        | Some t => typD ts t
+                        | Some t => typD t
                       end
   with
     | N n => n
@@ -398,7 +398,7 @@ Fixpoint my_inhabited t :=
 	  | _ => true
 	end.
 	
-Definition my_inhabited_sound : forall t ts, my_inhabited t = true -> Inhabited (typD ts t).
+Definition my_inhabited_sound : forall t, my_inhabited t = true -> Inhabited (typD t).
 Proof.
   intros.
   induction t.
